veric/CminorgenproofSIM.v
@@ -116,40 +116,80 @@ Lemma init_cores: forall (v1 v2 : val) (sig : signature) entrypoints
 (EP: In (v1, v2, sig) entrypoints)
   (vals1 : list val) (c1 : core_data) (m1 : mem) (j : meminj)
   (vals2 : list val) (m2 : mem)
- (CSM_Ini : make_initial_core CSharpMin_CompcertCoreSem ge v1 vals1 = Some c1)
+ (CSM_Ini : make_initial_core CSharpMin_core_sem ge v1 vals1 = Some c1)
  (Inj : Mem.inject j m1 m2)
  (VI: Forall2 (val_inject j) vals1 vals2)
  (HT: Forall2 Val.has_type vals2 (sig_args sig)),
 exists c2 : CMin_core,
-  make_initial_core CMin_CompcertCoreSem tge v2 vals2 = Some c2 /\
+  make_initial_core CMin_core_sem tge v2 vals2 = Some c2 /\
   match_cores c1 j c1 m1 c2 m2. 
+Proof. intros.
+  inversion CSM_Ini. unfold  CSharpMin_make_initial_core in H0. unfold ge in *. unfold tge in *.
+  destruct v1; inv H0.
+  remember (Int.eq_dec i Int.zero) as z; destruct z; inv H1. clear Heqz.
+  remember (Genv.find_funct_ptr (Genv.globalenv prog) b) as zz; destruct zz; inv H0. apply eq_sym in Heqzz.
+  (*
+                   remember (Genv.find_symbol (Genv.globalenv prog) CSharpMin_MainIdent) as z; destruct z; try inv H0.
+                   remember (Genv.find_funct_ptr  (Genv.globalenv prog) b) as zz; destruct zz; try inv H1. *)
+  exploit function_ptr_translated; eauto. intros [tf [FIND TR]].
+  unfold CMin_core_sem. simpl. unfold CMin_make_initial_core.
+(*
+  rewrite <- TprogMain. unfold transl_program in TRANSL.
+  econstructor; split.
+      destruct CMin_core_sem. simpl. destruct csem. simpl. 
+       econstructor.
+       unfold make_initial_core.
+  econstructor.
+  apply (Genv.init_mem_transf_partial2 _ _ _ TRANSL). eauto. 
+  simpl. fold tge. rewrite symbols_preserved.
+  replace (prog_main tprog) with (prog_main prog). eexact H0.
+  symmetry. unfold transl_program in TRANSL.
+  eapply transform_partial_program2_main; eauto.
+  eexact FIND. 
+  rewrite <- H2. apply sig_preserved; auto.
+  eapply match_callstate with (f := Mem.flat_inj (Mem.nextblock m0)) (cs := @nil frame).
+  auto.
+  eapply Genv.initmem_inject; eauto.
+  apply mcs_nil with (Mem.nextblock m0). apply match_globalenvs_init; auto. omega. omega.
+  instantiate (1 := gce). constructor.
+  red; auto. constructor. 
 (*
 v1 v2 vals1 (c1 : CSharpMin_core) m1 j vals2 m2 
       sig
-      (CSM_Ini : make_initial_core CSharpMin_CompcertCoreSem ge v1 vals1 = Some c1)
+      (CSM_Ini : make_initial_core CSharpMin_core_sem ge v1 vals1 = Some c1)
       (Inj : Mem.inject j m1 m2)
       (VI: Forall2 (val_inject j) vals1 vals2)
       (HT: Forall2 Val.has_type vals2 (sig_args sig)),
 exists cd : core_data,
   exists c2 : CMin_core,
-    make_initial_core CMin_CompcertCoreSem tge v2 vals2 = Some c2 /\
+    make_initial_core CMin_core_sem tge v2 vals2 = Some c2 /\
     match_cores cd j c1 m1 c2 m2.*)
 Proof.
-  intros. inv CSM_Ini.
+  intros. inv CSM_Ini. eexists. simpl. unfold CMin_make_initial_core. unfold tge.
+        rewrite <- TprogMain. rewrite <- Heqz.
   unfold  CSharpMin_make_initial_core in H0.
                               remember (Genv.find_symbol ge CSharpMin_MainIdent) as z; destruct z; try inv H0.
-                              remember (Genv.find_funct_ptr ge b) as zz; destruct zz; try inv H1.
+                             rewrite <- ProgMain in Heqz. unfold ge in Heqz. unfold tge in Heqz.
+                              rewrite <- (symbols_preserved _ _ TRANSL) in Heqz. 
+                              remember (Genv.find_funct_ptr ge b) as zz; destruct zz; try inv H1. 
+                              apply eq_sym in Heqzz.  unfold ge in Heqzz.
+                              destruct (Genv.find_funct_ptr_transf_partial2 _ _  _ TRANSL b Heqzz) as [tf  [Htf TransF]].
                               remember (Csharpminor.funsig f) as fs; destruct fs.
                               destruct sig_args; try inv H0.
                               destruct sig_res; try inv H1.
                               destruct t; try inv H0.
-  apply eq_sym in Heqzz.
-  destruct (function_ptr_translated _ _ TRANSL _ _ Heqzz) as [tf [FIND TR]].  
+(*  apply eq_sym in Heqzz.*)
+  destruct (function_ptr_translated _ _ TRANSL _ _ Heqzz) as [tff [FIND TR]].
+  rewrite FIND in Htf. inv Htf.  
     (*unfold core_data. exists (CSharpMin_Callstate f nil Csharpminor.Kstop).*)
    eexists.
   split.
   (*make_initial_core*)
-      simpl. unfold CMin_make_initial_core.
+      simpl. unfold CMin_make_initial_core. unfold tge.
+        rewrite <- TprogMain. rewrite <- Heqz.
+  rewrite (symbols_preserved _ _ TRANSL).
+          rewrite 
+          assert (Z:= sig_preserved _ _ _ TR). apply symbols_preserved; assumption.
       unfold ge in *. assert (ID: CMin_MainIdent = CSharpMin_MainIdent). admit. rewrite ID in *. 
               assert (X: Genv.find_symbol tge CSharpMin_MainIdent =  Genv.find_symbol (Genv.globalenv prog) CSharpMin_MainIdent).
                  apply symbols_preserved; assumption.
@@ -171,14 +211,14 @@ Proof.
 omega. omega.
   instantiate (1 := gce). constructor.
   red; auto. constructor.  econstructor.
-          econstructor.*)
+          econstructor.*)*)
 Admitted.
 
 Lemma MC_safely_halted: forall (cd : core_data) (j : meminj) (c1 : CSharpMin_core) (m1 : mem)
   (c2 : CMin_core) (m2 : mem) (v1 : int),
 match_cores cd j c1 m1 c2 m2 ->
-safely_halted CSharpMin_CompcertCoreSem ge c1 = Some v1 ->
-safely_halted CMin_CompcertCoreSem tge c2 = Some v1 /\ Mem.inject j m1 m2.
+safely_halted CSharpMin_core_sem ge c1 = Some v1 ->
+safely_halted CMin_core_sem tge c2 = Some v1 /\ Mem.inject j m1 m2.
 Proof.
   intros.
   inv H; simpl in *; inv H0.
@@ -190,13 +230,13 @@ Qed.
 Lemma MC_at_external: forall (cd : core_data) (j : meminj) (st1 : CSharpMin_core) (m1 : mem)
   (st2 : CMin_core) (m2 : mem) (e : external_function) (vals1 : list val) sig,
 (cd = st1 /\ match_cores cd j st1 m1 st2 m2) ->
-at_external CSharpMin_CompcertCoreSem st1 = Some (e, sig, vals1) ->
+at_external CSharpMin_core_sem st1 = Some (e, sig, vals1) ->
 Mem.inject j m1 m2 /\
 Events.meminj_preserves_globals ge j /\
 (exists vals2 : list val,
    Forall2 (val_inject j) vals1 vals2 /\
    Forall2 Val.has_type vals2 (sig_args sig) /\
-   at_external CMin_CompcertCoreSem st2 = Some (e, sig, vals2)).
+   at_external CMin_core_sem st2 = Some (e, sig, vals2)).
 Proof.
   intros. destruct H; subst.
   inv H1; simpl in *; inv H0.
@@ -214,7 +254,7 @@ Lemma MC_after_external:forall (d : core_data) (j j' : meminj) (st1 : core_data)
   (m1 : mem) (e : external_function) (vals1 : list val) (ret1 : val)
   (m1' m2 m2' : mem) (ret2 : val) (sig : signature),
 d = st1 /\ match_cores d j st1 m1 st2 m2 ->
-at_external CSharpMin_CompcertCoreSem st1 = Some (e, sig, vals1) ->
+at_external CSharpMin_core_sem st1 = Some (e, sig, vals1) ->
 Events.meminj_preserves_globals ge j ->
 inject_incr j j' ->
 Events.inject_separated j j' m1 m2 ->
@@ -228,8 +268,8 @@ Val.has_type ret2 (proj_sig_res sig) ->
 exists st1' : core_data,
   exists st2' : CMin_core,
     exists d' : core_data,
-      after_external CSharpMin_CompcertCoreSem (Some ret1) st1 = Some st1' /\
-      after_external CMin_CompcertCoreSem (Some ret2) st2 = Some st2' /\
+      after_external CSharpMin_core_sem (Some ret1) st1 = Some st1' /\
+      after_external CMin_core_sem (Some ret2) st2 = Some st2' /\
       d' = st1' /\ match_cores d' j' st1' m1' st2' m2'. 
 Proof. intros.
   destruct (MC_at_external _ _ _ _ _ _ _ _ _ H H0) as [_ [_ [vals2 [ValsInj [vals2Typ AtExt2]]]]].
@@ -572,7 +612,7 @@ Proof. intros.
      (*exists  (CSharpMin_Callstate fd vargs (Csharpminor.Kcall optid f e lenv tk)).
      left.*) econstructor; eauto. eapply match_Kcall with (cenv' := cenv); eauto.
             simpl; trivial.
-      admit. admit. (*These are the new conditions in rulenv MC_Callstate*)
+      admit. admit. (*These are the new conditions in rule MC_Callstate*)
 Qed.
 
 Lemma MS_step_case_Builtin:
@@ -1187,7 +1227,7 @@ Lemma MS_match_callstack_alloc_variables_rec:
   /\ (forall b, Mem.valid_block m b -> f' b = f b)
   /\ (forall b b' d', f b = None -> f' b = Some (b',d') -> b' = sp)
   /\ forall j',  inject_incr f' j' -> Events.inject_separated f' j' m' tm -> Events.inject_separated f' j' m tm .
-Proof.
+Proof. clear core_data. 
   intros until atk. intros VALID BOUNDS PERM NOOV.
   induction 1.
   (* base case *)
@@ -1205,7 +1245,7 @@ Proof.
     intros. eapply DEFINED. simpl. right. eauto.
   assert (exists tv, te!(for_var id) = Some tv).
     assert (te!(for_var id) <> None). eapply DEFINED. simpl; left; auto.
-    destruct (te!(for_var id)). exists v; auto. exfalso. apply H1.  trivial. (*congruence. won;'t worlk here all of a sudden*)
+    destruct (te!(for_var id)). exists v; auto. congruence. 
   destruct H1 as [tv TEID].
   assert (sz1 <= fn_stackspace tf). eapply assign_variables_incr; eauto. 
   exploit MS_match_callstack_alloc_variable; eauto with coqlib.
@@ -1256,7 +1296,7 @@ Lemma MS_match_callstack_alloc_variables:
   /\ (forall b, Mem.valid_block m b -> f' b = f b)
   /\ (forall b b' d', f b = None -> f' b = Some (b',d') -> b' = sp)
   /\ forall j',  inject_incr f' j' -> Events.inject_separated f' j' m' tm' -> Events.inject_separated f j' m tm.
-Proof.
+Proof. clear core_data.
   intros.
   unfold build_compilenv in H.
 assert (AR: exists f',
@@ -1293,7 +1333,7 @@ exists f' ; intuition.
             assert (j' b = Some (b0,z)). apply (H6 _ _ _ Heqz). 
              rewrite H9 in H10; inv H10.
              assert (Z:= SP _ _ _ H8 Heqz); subst.
-             split; intros N. rewrite (VB1 _ N) in Heqz. rewrite Heqz in H8. inv H8. (*congruence again doesnt work here*)
+             split; intros N. rewrite (VB1 _ N) in Heqz. congruence.
              eapply (Mem.fresh_block_alloc _ _ _ _ _ H3 N).
   (*None*) assert (HH:= SEP _ H6 H7).
                      destruct (HH _ _ _ Heqz H9).
@@ -1317,7 +1357,7 @@ Lemma MS_var_set_self_correct_scalar:
 (********* The following 2 conditions are new*****)
    /\ (forall b, Mem.valid_block m b -> Mem.valid_block m' b) (* actually <-> holds*)
   /\ (forall b, Mem.valid_block tm b -> Mem.valid_block tm' b). (* actually <-> holds*)
-Proof.
+Proof. clear core_data.
   intros until k. 
   intros VS MCS VINJ MINJ ASG VAL.
   unfold var_set_self in VS. inv ASG. 
@@ -1327,14 +1367,10 @@ Proof.
     inv MCS. inv MENV. auto.
   assert (EVAR: eval_expr tge (Vptr sp Int.zero) te tm (Evar (for_var id)) tv).
     constructor. auto.
-  revert VS; inv MV; intro VS; inv VS; inv H (*; try congruence. *).
-         Focus 2. rewrite H3 in H8; inv H8. 
-         Focus 3.  rewrite H3 in H5; inv H5.
-         Focus 3.  rewrite H3 in H5; inv H5.
-         Focus 3.  rewrite H3 in H5; inv H5.
+  revert VS; inv MV; intro VS; inv VS; inv H; try congruence. 
   (* var_local *)
-  rewrite H3 in H8; inv H8. (*assert (b0 = b) by congruence. subst b0. 
-  assert (chunk0 = chunk) by congruence. subst chunk0.*)
+  assert (b0 = b) by congruence. subst b0. 
+  assert (chunk0 = chunk) by congruence. subst chunk0.
   exists tm.
   split. apply corestep_star_zero. 
   split. eapply Mem.store_unmapped_inject; eauto. 
@@ -1343,7 +1379,7 @@ Proof.
     apply match_callstack_extensional with (PTree.set (for_var id) tv te).
     intros. repeat rewrite PTree.gsspec.
     destruct (peq (for_var id0) (for_var id)). congruence. auto.
-    intros. rewrite PTree.gso; auto. unfold for_temp, for_var. intros N. inv N. (* congruence.*)
+    intros. rewrite PTree.gso; auto. unfold for_temp, for_var. congruence. 
     eapply match_callstack_store_local; eauto.
   split; intros; trivial. 
     (*apply prop_ext.
@@ -1398,7 +1434,7 @@ Lemma MS_var_set_self_correct_array:
     Events.inject_separated f f' m tm  /\
     (forall b, Mem.valid_block m b -> Mem.valid_block m' b) (* actually <-> holds*)
   /\ (forall b, Mem.valid_block tm b -> Mem.valid_block tm' b). 
-Proof.
+Proof. clear core_data.
   intros until k. 
   intros VS MCS VINJ MINJ KIND MEMCPY VAL.
   assert (MV: match_var prog f id e m te sp cenv!!id).
@@ -1660,13 +1696,16 @@ exists c2' : CMin_core,
         inject_incr j j' /\
         (*again, have inject-sparatated here, as per definition of match relation*) 
          Events.inject_separated j j' m tm /\
-  exists c',
-        inj_match_states_star unit match_cores MC_measure (tt,c') j'
+         match_cores  (CSharpMin_State f (Csharpminor.fn_body f) k e empty_temp_env)  j'
            (CSharpMin_State f (Csharpminor.fn_body f) k e empty_temp_env) m2 c2' m2'.
+(*  exists c',
+        inj_match_states_star unit match_cores MC_measure (tt,c') j'
+           (CSharpMin_State f (Csharpminor.fn_body f) k e empty_temp_env) m2 c2' m2'.*)
 Proof. intros.
   generalize EQ; clear EQ; unfold transl_function.
   caseEq (build_compilenv gce f). intros ce sz BC.
-  destruct (zlenv sz Int.max_unsigned); try congruence.
+  destruct (zle sz Int.max_unsigned). Focus 2. intros. exfalso. clear core_data.  congruence. (*core data versus congruence bug; Xavier's proof has 
+             destruct (zle sz Int.max_unsigned); try congruence here....*)
   intro TRBODY.
   generalize TRBODY; intro TMP. monadInv TMP.
   set (tf := mkfunction (Csharpminor.fn_sig f) 
@@ -1690,8 +1729,6 @@ Proof. intros.
   simpl in *.
   exists j'. split. assumption.
   split. assumption.
-  exists (CSharpMin_State f(Csharpminor.fn_body f) k e empty_temp_env).
-  left.
   econstructor. eexact TRBODY. eauto. eexact MINJ2. 
   eexact MCS2.
   inv MK; simpl in ISCC; contradiction || econstructor; eauto.
@@ -1709,21 +1746,19 @@ forall j m tm cs f e lenv k tk ty cenv v tv optid
 exists c2' : CMin_core,
   exists m2' : mem,
        corestep_plus CMin_core_sem tge (CMin_Returnstate tv tk) tm c2' m2'  /\
-    exists c', 
-       inj_match_states_star unit match_cores MC_measure (tt,c') j
+       match_cores  (CSharpMin_State f Csharpminor.Sskip k e (set_optvar optid v lenv)) j
              (CSharpMin_State f Csharpminor.Sskip k e (set_optvar optid v lenv)) m c2' m2' .
 Proof. intros.
   inv MK. simpl.
   eexists; eexists; split.
        eapply corestep_plus_one. eapply CompCertStep_CMin_corestep'. econstructor; eauto. reflexivity.
   simpl.
-  exists  (CSharpMin_State f Csharpminor.Sskip k e (set_optvar optid v lenv)).
-    left. unfold set_optvar. destruct optid; simpl option_map; econstructor; eauto.              
+  unfold set_optvar. destruct optid; simpl option_map; econstructor; eauto.              
          eapply match_callstack_set_temp; eauto. 
 Qed. 
 
 Lemma MS_step: forall (c1 : core_data) (m1 : mem) (c1' : core_data) (m1' : mem),
-corestep CSharpMin_CompcertCoreSem ge c1 m1 c1' m1' ->
+corestep CSharpMin_core_sem ge c1 m1 c1' m1' ->
 forall (c2 : CMin_core) (m2 : mem) (j : meminj),
 match_cores c1 j c1 m1 c2 m2 ->
 (exists c2' : CMin_core,
@@ -1731,7 +1766,7 @@ match_cores c1 j c1 m1 c2 m2 ->
      exists j' : meminj,
        inject_incr j j' /\
        Events.inject_separated j j' m1 m2 /\
-       corestep_plus CMin_CompcertCoreSem tge c2 m2 c2' m2' /\
+       corestep_plus CMin_core_sem tge c2 m2 c2' m2' /\
        match_cores c1' j' c1' m1' c2' m2') \/
 (MC_measure c1' < MC_measure c1)%nat /\ match_cores c1' j c1' m1' c2 m2.
 Proof.
@@ -2005,8 +2040,8 @@ Proof.
       rename m1 into m. rename m2 into tm. rename f0 into f. rename e0 into e.
       rename m0 into m1. rename args into vargs. rename m1' into m2.
       rename k0 into tk. rename args0 into targs. 
-      destruct (MS_step_case_InternalCall _ _ _ _ _ _ _ _ _ _ _ _ _ _ H2 H3 H5 MINJ MCS MK ISCC ARGSINJ EQ) as [c2' [m2' [cstepPlus [j' [InjIncr [InjSep [c' MS]]]]]]].
-      exists c2'. exists m2'. exists (tt,c'). exists j'. auto.
+      destruct (MS_step_case_InternalCall _ _ _ _ _ _ _ _ _ _ _ _ _ _ H2 H3 H5 MINJ MCS MK ISCC ARGSINJ EQ) as [c2' [m2' [cstepPlus [j' [InjIncr [InjSep MS]]]]]].
+      left. exists c2'. exists m2'. exists j'. auto.
 (* external call *)
       destruct c1; simpl in *; try inv H0. inv H. 
    (*nothing to show here - cf corestep not at external *) 
@@ -2025,1136 +2060,49 @@ Proof.
       destruct c1'; simpl in *; try inv H3. 
       inv MSTATE. 
       destruct c2; simpl in *; try inv H5. rename m1' into m. rename m2 into tm. rename f0 into f. rename e0 into e. rename k into tk. rename k0 into k. rename v into tv. rename v0 into v.
-      destruct (MS_step_case_Return _ _ _ _ _ _ _ _ _ _ _ _ tv optid MINJ MCS MK RESINJ) as [c2' [m2' [cstepPlus [c' MS]]]]. 
-      exists c2'. exists m2'. exists (tt,c'). exists j.
+      destruct (MS_step_case_Return _ _ _ _ _ _ _ _ _ _ _ _ tv optid MINJ MCS MK RESINJ) as [c2' [m2' [cstepPlus MS]]]. 
+      left. exists c2'. exists m2'. exists j.
       split. apply inject_incr_refl.
       split. apply inject_separated_same_meminj.
       auto. 
 Qed.
+
 Goal forall entrypoints, 
-Sim_inj.Forward_simulation_inject _ _ CSharpMin_CompcertCoreSem 
-   CMin_CompcertCoreSem ge tge entrypoints.
+Sim_inj.Forward_simulation_inject _ _ CSharpMin_core_sem 
+   CMin_core_sem ge tge entrypoints.
 Proof.
 intros. apply inj_simulation_star with (match_states:=match_cores)(measure:=MC_measure).
    intros. eapply (init_cores _ _ _ entrypoints); eauto.
    apply MC_safely_halted.
    apply MC_at_external.
    apply  MC_after_external.
+   apply MS_step.
+Qed.
 
-
-Goal forall entrypoints, 
-Sim_inj.Forward_simulation_inject _ _ CSharpMin_CompcertCoreSem 
-   CMin_CompcertCoreSem ge tge entrypoints.
+Theorem transl_program_correct: forall entrypoints, 
+Sim_inj.Forward_simulation_inject _ _ CSharpMin_core_sem 
+   CMin_core_sem ge tge entrypoints.
 Proof.
 intros. apply inj_simulation_star with (match_states:=match_cores)(measure:=MC_measure).
    intros. eapply (init_cores _ _ _ entrypoints); eauto.
    apply MC_safely_halted.
    apply MC_at_external.
    apply  MC_after_external.
-Admitted.
+  apply MS_step.
+Qed.
 
-
-(******************************Functions required for internal call rule*****************************)
-(****These extend the original lemmas by additional guarantees of the (now exposed) memory injections, in order
-    for the overall lemma for internal calls to establish the inject_separated fact******************************)
-Lemma MS_match_callstack_alloc_variable:
-  forall atk id lv cenv sz cenv' sz' tm sp e tf m m' b te lenv lo cs f tv,
-  assign_variablenv atk (id, lv) (cenv, sz) = (cenv', sz') ->
-  Mem.valid_block tm sp ->
-  (forall ofs k p,
-    Mem.perm tm sp ofs k p -> 0 <= ofs < tf.(fn_stackspace)) ->
-  Mem.range_perm tm sp 0 tf.(fn_stackspace) Cur Freeablenv ->
-  tf.(fn_stackspace) <= Int.max_unsigned ->
-  Mem.alloc m 0 (sizeof lv) = (m', b) ->
-  match_callstack prog f m tm 
-                  (Frame cenv tf e lenv te sp lo (Mem.nextblock m) :: cs)
-                  (Mem.nextblock m) (Mem.nextblock tm) ->
-  Mem.inject f m tm ->
-  0 <= sz -> sz' <= tf.(fn_stackspace) ->
-  (forall b delta ofs k p,
-     f b = Some(sp, delta) -> Mem.perm m b ofs k p -> ofs + delta < sz) ->
-  e!id = None ->
-  te!(for_var id) = Some tv ->
-  exists f',
-     inject_incr f f'
-  /\ Mem.inject f' m' tm
-  /\ match_callstack prog f' m' tm
-                     (Frame cenv' tf (PTree.set id (b, lv) e) lenv te sp lo (Mem.nextblock m') :: cs)
-                     (Mem.nextblock m') (Mem.nextblock tm)
-  /\ (forall b delta ofs k p,
-      f' b = Some(sp, delta) -> Mem.perm m' b ofs k p -> ofs + delta < sz') 
-(****************The following three conditions are new******************)
-  /\ (forall b, Mem.valid_block m b -> f' b = f b)
-  /\ (forall b b' d', f b = None -> f' b = Some (b',d') -> b' = sp)
-  /\ forall j',  inject_incr f' j' -> Events.inject_separated f' j' m' tm -> Events.inject_separated f' j' m tm.
+Theorem transl_program_correct_CompcertCoreSem: forall entrypoints, 
+Sim_inj.Forward_simulation_inject _ _ CSharpMin_CompcertCoreSem
+   CMin_CompcertCoreSem ge tge entrypoints.
 Proof.
-  intros until tv. intros ASV VALID BOUNDS PERMS NOOV ALLOC MCS INJ LO HI RANGE E TE.
-  generalize ASV. unfold assign_variable. 
-  caseEq lv.
-  (* 1. lv = LVscalar chunk *)
-  intros chunk LV. case (Identset.mem id atk).
-  (* 1.1 info = Var_stack_scalar chunk ofs *)
-    set (ofs := align sz (size_chunk chunk)).
-    intro EQ; injection EQ; intros; clear EQ. rewrite <- H0.
-    generalize (size_chunk_pos chunk); intro SIZEPOS.
-    generalize (align_lenv sz (size_chunk chunk) SIZEPOS). fold ofs. intro SZOFS.
-    exploit Mem.alloc_left_mapped_inject.
-      eauto. eauto. eauto. 
-      instantiate (1 := ofs). omega.
-      intros. exploit BOUNDS; eauto. omega. 
-      intros. apply Mem.perm_implies with Freeable; auto with mem. apply Mem.perm_cur. 
-      apply PERMS. rewrite LV in H1. simpl in H1. omega.
-      rewrite LV; simpl. rewrite Zminus_0_r. unfold ofs. 
-      apply inj_offset_aligned_var.
-      intros. generalize (RANGE _ _ _ _ _ H1 H2). omega. 
-    intros [f1 [MINJ1 [INCR1 [SAME OTHER]]]].
-    exists f1; split. auto. split. auto. split. 
-    eapply match_callstack_alloc_left; eauto.
-    rewrite <- LV; auto. 
-    rewrite SAME; constructor.
-  split.
-    intros. exploit Mem.perm_alloc_inv; eauto. destruct (zeq b0 b).
-    subst b0. assert (delta = ofs) by congruence. subst delta.  
-    rewrite LV. simpl. omega.
-    intro. rewrite OTHER in H1; eauto. generalize (RANGE _ _ _ _ _ H1 H3). omega. 
-  assert (XX: forall b0 : Values.block, Mem.valid_block m b0 -> f1 b0 = f b0).
-     intros b0; intros. destruct (eq_block b0 b); subst. 
-                     exfalso. apply (Mem.fresh_block_alloc _ _ _ _ _ ALLOC H1).
-                  apply (OTHER _ n).
-   split; trivial.
-   split; intros. destruct (eq_block b0 b); subst. rewrite SAME in H2. inv H2. trivial.
-                         rewrite (OTHER _ n) in H2. congruence. 
-     intros. intros bb; intros.
-     destruct (H2 _ _ _ H3 H4). split; trivial. intros N. apply H5. eapply Mem.valid_block_alloc; eauto.
-  (* 1.2 info = Var_local chunk *)
-    intro EQ; injection EQ; intros; clear EQ. subst sz'. rewrite <- H0.
-    exploit Mem.alloc_left_unmapped_inject; eauto.
-    intros [f1 [MINJ1 [INCR1 [SAME OTHER]]]].
-    exists f1; split. auto. split. auto. split.
-      eapply match_callstack_alloc_left; eauto.  
-      rewrite <- LV; auto.
-      rewrite SAME; constructor.
-   split.
-      intros. exploit Mem.perm_alloc_inv; eauto. destruct (zeq b0 b).
-      subst b0. congruence.
-      rewrite OTHER in H; eauto.
-  assert (XX: forall b0 : Values.block, Mem.valid_block m b0 -> f1 b0 = f b0).
-     intros b0; intros. destruct (eq_block b0 b); subst. 
-                     exfalso. apply (Mem.fresh_block_alloc _ _ _ _ _ ALLOC H).
-                  apply (OTHER _ n).
-   split; trivial.
-   split; intros. destruct (eq_block b0 b); subst. rewrite SAME in H1. inv H1.
-                         rewrite (OTHER _ n) in H1. congruence. 
-   intros bb; intros.
-     destruct (H1 _ _ _ H2 H3). split; trivial. intros N. apply H4. eapply Mem.valid_block_alloc; eauto.
-  (* 2 info = Var_stack_array ofs *)
-  intros dim al LV EQ. injection EQ; clear EQ; intros. rewrite <- H.
-  assert (0 <= Zmax 0 dim). apply Zmax1. 
-  generalize (align_lenv sz (array_alignment dim) (array_alignment_pos dim)). intro.
-  set (ofs := align sz (array_alignment dim)) in *.
-  exploit Mem.alloc_left_mapped_inject. eauto. eauto. eauto. 
-    instantiate (1 := ofs). 
-    generalize Int.min_signed_neg. omega.
-    intros. exploit BOUNDS; eauto. generalize Int.min_signed_neg. omega.
-    intros. apply Mem.perm_implies with Freeable; auto with mem. apply Mem.perm_cur.
-    apply PERMS. rewrite LV in H3. simpl in H3. omega.
-    rewrite LV; simpl. rewrite Zminus_0_r. unfold ofs. 
-    apply inj_offset_aligned_array'.
-    intros. generalize (RANGE _ _ _ _ _ H3 H4). omega. 
-  intros [f1 [MINJ1 [INCR1 [SAME OTHER]]]].
-  exists f1; split. auto. split. auto. split. 
-    subst cenv'. eapply match_callstack_alloc_left; eauto.
-    rewrite <- LV; auto. 
-    rewrite SAME; constructor.
-  split.
-    intros. exploit Mem.perm_alloc_inv; eauto. destruct (zeq b0 b).
-    subst b0. assert (delta = ofs) by congruence. subst delta. 
-    rewrite LV. simpl. omega.
-    intro. rewrite OTHER in H3; eauto. generalize (RANGE _ _ _ _ _ H3 H5). omega. 
-  assert (XX: forall b0 : Values.block, Mem.valid_block m b0 -> f1 b0 = f b0).
-     intros b0; intros. destruct (eq_block b0 b); subst. 
-                     exfalso. apply (Mem.fresh_block_alloc _ _ _ _ _ ALLOC H3).
-                  apply (OTHER _ n).
-   split; trivial.
-   split; intros. destruct (eq_block b0 b); subst. rewrite SAME in H4. inv H4. trivial.
-                         rewrite (OTHER _ n) in H4. congruence. 
-   intros bb; intros.
-     destruct (H4 _ _ _ H5 H6). split; trivial. intros N. apply H7. eapply Mem.valid_block_alloc; eauto.
-Qed.
-
-Lemma MS_match_callstack_alloc_variables_rec:
-  forall tm sp cenv' tf lenv te lo cs atk,
-  Mem.valid_block tm sp ->
-  (forall ofs k p,
-    Mem.perm tm sp ofs k p -> 0 <= ofs < tf.(fn_stackspace)) ->
-  Mem.range_perm tm sp 0 tf.(fn_stackspace) Cur Freeablenv ->
-  tf.(fn_stackspace) <= Int.max_unsigned ->
-  forall e m vars e' m',
-  alloc_variables e m vars e' m' ->
-  forall f cenv sz,
-  assign_variables atk vars (cenv, sz) = (cenv', tf.(fn_stackspace)) ->
-  match_callstack prog f m tm 
-                  (Frame cenv tf e lenv te sp lo (Mem.nextblock m) :: cs)
-                  (Mem.nextblock m) (Mem.nextblock tm) ->
-  Mem.inject f m tm ->
-  0 <= sz ->
-  (forall b delta ofs k p,
-     f b = Some(sp, delta) -> Mem.perm m b ofs k p -> ofs + delta < sz) ->
-  (forall id lv, In (id, lv) vars -> te!(for_var id) <> None) ->
-  list_norepet (List.map (@fst ident var_kind) vars) ->
-  (forall id lv, In (id, lv) vars -> e!id = None) ->
-  exists f',
-     inject_incr f f'
-  /\ Mem.inject f' m' tm
-  /\ match_callstack prog f' m' tm
-                     (Frame cenv' tf e' lenv te sp lo (Mem.nextblock m') :: cs)
-                     (Mem.nextblock m') (Mem.nextblock tm)
-(****************The following three conditions are new******************)
-(*** Note that in the third clause, we only "step" from m' to m ***************)
-  /\ (forall b, Mem.valid_block m b -> f' b = f b)
-  /\ (forall b b' d', f b = None -> f' b = Some (b',d') -> b' = sp)
-  /\ forall j',  inject_incr f' j' -> Events.inject_separated f' j' m' tm -> Events.inject_separated f' j' m tm .
-Proof.
-  intros until atk. intros VALID BOUNDS PERM NOOV.
-  induction 1.
-  (* base case *)
-  intros. simpl in H. inversion H; subst cenv sz.
-  exists f. split. apply inject_incr_refl. split. auto. split. auto.
-    split; trivial.
-    split; trivial. intros. congruence.
-  (* inductive case *)
-  intros until sz.
-  change (assign_variables atk ((id, lv) :: vars) (cenv, sz))
-  with (assign_variables atk vars (assign_variablenv atk (id, lv) (cenv, sz))).
-  caseEq (assign_variablenv atk (id, lv) (cenv, sz)).
-  intros cenv1 sz1 ASV1 ASVS MATCH MINJ SZPOS BOUND DEFINED NOREPET UNDEFINED.
-  assert (DEFINED1: forall id0 lv0, In (id0, lv0) vars -> te!(for_var id0) <> None).
-    intros. eapply DEFINED. simpl. right. eauto.
-  assert (exists tv, te!(for_var id) = Some tv).
-    assert (te!(for_var id) <> None). eapply DEFINED. simpl; left; auto.
-    destruct (te!(for_var id)). exists v; auto. congruence.
-  destruct H1 as [tv TEID].
-  assert (sz1 <= fn_stackspace tf). eapply assign_variables_incr; eauto. 
-  exploit MS_match_callstack_alloc_variable; eauto with coqlib.
-  intros [f1 [INCR1 [INJ1 [MCS1 [BOUND1 [VB [SP SEP]]]]]]].
-  exploit IHalloc_variables; eauto. 
-  apply Zle_trans with sz; auto. eapply assign_variable_incr; eauto.
-  inv NOREPET; auto.
-  intros. rewrite PTree.gso. eapply UNDEFINED; eauto with coqlib.
-  simpl in NOREPET. inversion NOREPET. red; intro; subst id0.
-  elim H5. change id with (fst (id, lv0)). apply List.in_map. auto.
-  intros [f2 [INCR2 [INJ2 [MCS2 [VBF2 [SP2 SEP2]]]]]].
-  assert (X: forall b : Values.block, Mem.valid_block m b -> f2 b = f b).
-           intros. rewrite <- (VB _ H2). apply VBF2. eapply Mem.valid_block_alloc; eauto.
-  assert (Y:  (forall (b b' : Values.block) (d' : Z), f b = None -> f2 b = Some (b', d') -> b' = sp)).
-       clear MCS2 BOUND1 MCS1 DEFINED1 SEP SEP2 IHalloc_variables UNDEFINED.
-          intros. remember (f1 b) as z. destruct z; apply eq_sym in Heqz.
-              destruct p.  assert (Z1 := SP _ _ _ H2 Heqz). subst.
-                 apply INCR2 in Heqz. rewrite Heqz in H3. inv H3. trivial.
-             apply (SP2 _ _ _ Heqz H3).
-  exists f2 ; intuition.
-    eapply inject_incr_trans; eauto.
-    intros b; intros. destruct (H3 _ _ _ H4 H5). split; trivial.
-     intros N. apply H6. apply (Mem.valid_block_alloc _ _ _ _ _ H) in N.
-              eapply allocvars_blocks_valid; eauto.
-Qed. 
-
-Lemma MS_match_callstack_alloc_variables:
-  forall fn cenv tf m e m' tm tm' sp f cs targs,
-  build_compilenv gce fn = (cenv, tf.(fn_stackspace)) ->
-  tf.(fn_stackspace) <= Int.max_unsigned ->
-  list_norepet (fn_params_names fn ++ fn_vars_names fn) ->
-  alloc_variables Csharpminor.empty_env m (fn_variables fn) e m' ->
-  Mem.alloc tm 0 tf.(fn_stackspace) = (tm', sp) ->
-  match_callstack prog f m tm cs (Mem.nextblock m) (Mem.nextblock tm) ->
-  Mem.inject f m tm ->
-  let tparams := List.map for_var (fn_params_names fn) in
-  let tvars := List.map for_var (fn_vars_names fn) in
-  let ttemps := List.map for_temp (Csharpminor.fn_temps fn) in
-  let te := set_locals (tvars ++ ttemps) (set_params targs tparams) in
-  exists f',
-     inject_incr f f'
-  /\ Mem.inject f' m' tm'
-  /\ match_callstack prog f' m' tm'
-                     (Frame cenv tf e empty_temp_env te sp (Mem.nextblock m) (Mem.nextblock m') :: cs)
-                     (Mem.nextblock m') (Mem.nextblock tm') 
-(****************The following three conditions are new******************)
-(* In the third clause, we now stepfrom  m' to m, and also from f' to f and from tm' to tm******************)
-  /\ (forall b, Mem.valid_block m b -> f' b = f b)
-  /\ (forall b b' d', f b = None -> f' b = Some (b',d') -> b' = sp)
-  /\ forall j',  inject_incr f' j' -> Events.inject_separated f' j' m' tm' -> Events.inject_separated f j' m tm.
-Proof.
-  intros.
-  unfold build_compilenv in H.
-assert (AR: exists f',
-     inject_incr f f'
-  /\ Mem.inject f' m' tm'
-  /\ match_callstack prog f' m' tm'
-                     (Frame cenv tf e empty_temp_env te sp (Mem.nextblock m) (Mem.nextblock m') :: cs)
-                     (Mem.nextblock m') (Mem.nextblock tm') 
-  /\ (forall b, Mem.valid_block m b -> f' b = f b)
-  /\ (forall b b' d', f b = None -> f' b = Some (b',d') -> b' = sp)
-  /\ forall j',  inject_incr f' j' -> Events.inject_separated f' j' m' tm' -> Events.inject_separated f' j' m tm').
-  eapply MS_match_callstack_alloc_variables_rec; eauto with mem.
-  red; intros. eapply Mem.perm_alloc_2; eauto. 
-  eapply match_callstack_alloc_right; eauto.
-  eapply Mem.alloc_right_inject; eauto. omega. 
-  intros. elim (Mem.valid_not_valid_diff tm sp sp); eauto with mem.
-  eapply Mem.valid_block_inject_2; eauto.
-  intros. unfold te. apply set_locals_params_defined.
-  elim (in_app_or _ _ _ H6); intros.
-  apply in_or_app; left. unfold tparams. apply List.in_map.
-  change id with (fst (id, lv)). apply List.in_map. auto.
-  apply in_or_app; right. apply in_or_app; left. unfold tvars. apply List.in_map. 
-  change id with (fst (id, lv)). apply List.in_map; auto.
-  (* norepet *)
-  unfold fn_variables. rewrite List.map_app. assumption.
-  (* undef *)
-  intros. unfold empty_env. apply PTree.gempty.
-
-destruct AR as  [f' [INC [INJ [MC [VB1 [SP SEP]]]]]].
-exists f' ; intuition.
-  intros b; intros.
-  remember (f' b) as z; destruct z; apply eq_sym in Heqz.
-  (*Some p*) destruct p.
-            assert (j' b = Some (b0,z)). apply (H6 _ _ _ Heqz). 
-             rewrite H9 in H10; inv H10.
-             assert (Z:= SP _ _ _ H8 Heqz); subst.
-             split; intros N. rewrite (VB1 _ N) in Heqz. congruence.
-             eapply (Mem.fresh_block_alloc _ _ _ _ _ H3 N).
-  (*None*) assert (HH:= SEP _ H6 H7).
-                     destruct (HH _ _ _ Heqz H9).
-                     split; trivial. 
-                     intros N. apply H11. eapply Mem.valid_block_alloc; eauto. 
-Qed.
-
-Lemma MS_var_set_self_correct_scalar:
-  forall cenv id s a f tf e lenv te sp lo hi m cs tm tv v m' fn k,
-  var_set_self cenv id s = OK a ->
-  match_callstack prog f m tm (Frame cenv tf e lenv te sp lo hi :: cs) (Mem.nextblock m) (Mem.nextblock tm) ->
-  val_inject f v tv ->
-  Mem.inject f m tm ->
-  exec_assign ge e m id v m' ->
-  te!(for_var id) = Some tv ->
-  exists tm',
-    corestep_star CMin_core_sem tge (CMin_State fn a k (Vptr sp Int.zero) te) tm
-                                    (CMin_State fn s k (Vptr sp Int.zero) te) tm' /\
-    Mem.inject f m' tm' /\
-    match_callstack prog f m' tm' (Frame cenv tf e lenv te sp lo hi :: cs) (Mem.nextblock m') (Mem.nextblock tm') 
-(********* The following 2 conditions are new*****)
-   /\ (forall b, Mem.valid_block m b -> Mem.valid_block m' b) (* actually <-> holds*)
-  /\ (forall b, Mem.valid_block tm b -> Mem.valid_block tm' b). (* actually <-> holds*)
-Proof.
-  intros until k. 
-  intros VS MCS VINJ MINJ ASG VAL.
-  unfold var_set_self in VS. inv ASG. 
-  assert (NEXTBLOCK: Mem.nextblock m' = Mem.nextblock m).
-    eapply Mem.nextblock_store; eauto.
-  assert (MV: match_var prog f id e m te sp cenv!!id).
-    inv MCS. inv MENV. auto.
-  assert (EVAR: eval_expr tge (Vptr sp Int.zero) te tm (Evar (for_var id)) tv).
-    constructor. auto.
-  revert VS; inv MV; intro VS; inv VS; inv H; try congruence.
-  (* var_local *)
-  assert (b0 = b) by congruence. subst b0.
-  assert (chunk0 = chunk) by congruence. subst chunk0.
-  exists tm.
-  split. apply corestep_star_zero. 
-  split. eapply Mem.store_unmapped_inject; eauto. 
-  rewrite NEXTBLOCK. 
-  split.
-    apply match_callstack_extensional with (PTree.set (for_var id) tv te).
-    intros. repeat rewrite PTree.gsspec.
-    destruct (peq (for_var id0) (for_var id)). congruence. auto.
-    intros. rewrite PTree.gso; auto. unfold for_temp, for_var; congruence.
-    eapply match_callstack_store_local; eauto.
-  split; intros; trivial. 
-    (*apply prop_ext.
-    split; intros. *) eapply Mem.store_valid_block_1; eauto.
-     (* eapply Mem.store_valid_block_2; eauto.*)
-  (* var_stack_scalar *)
-  assert (b0 = b) by congruence. subst b0.
-  assert (chunk0 = chunk) by congruence. subst chunk0.
-  assert (Mem.storev chunk m (Vptr b Int.zero) v = Some m'). assumption.
-  exploit make_store_correct.
-    eapply make_stackaddr_correct.
-    eauto. eauto. eauto. eauto. eauto. 
-  intros [tm' [tvrhs' [EVAL' [STORE' MEMINJ]]]].
-  exists tm'.
-  split. eapply corestep_star_trans.
-           eapply corestep_star_one. eapply CompCertStep_CMin_corestep'. econstructor. reflexivity.
-         simpl. 
-         eapply corestep_star_trans.
-           eapply corestep_star_one. eapply CompCertStep_CMin_corestep'. apply EVAL'. reflexivity. 
-         simpl.
-           eapply corestep_star_one. eapply CompCertStep_CMin_corestep. constructor. reflexivity.
-  split. trivial.
-  split.
-    rewrite NEXTBLOCK. rewrite (nextblock_storev _ _ _ _ _ STORE'). 
-    eapply match_callstack_storev_mapped; eauto.
-  split; intros. 
-    (*apply prop_ext; split; intros. *) eapply Mem.store_valid_block_1; eauto.
-           (* eapply Mem.store_valid_block_2; eauto.  *)
-    inv EVAL'.  (*apply prop_ext; split; intros.  *) eapply storev_valid_block_1; eauto.
-                             (*eapply storev_valid_block_2; eauto.   *)
-Qed.
-
-Lemma MS_var_set_self_correct_array:
-  forall cenv id s a f tf e lenv te sp lo hi m cs tm tv b v sz al m' fn k,
-  var_set_self cenv id s = OK a ->
-  match_callstack prog f m tm (Frame cenv tf e lenv te sp lo hi :: cs) (Mem.nextblock m) (Mem.nextblock tm) ->
-  val_inject f v tv ->
-  Mem.inject f m tm ->
-  PTree.get id e = Some(b, Varray sz al) ->
-  Events.extcall_memcpy_sem sz (Zmin al 4) ge
-                             (Vptr b Int.zero :: v :: nil) m Events.E0 Vundef m' ->
-  te!(for_var id) = Some tv ->
-  exists f', exists tm',
-    corestep_star CMin_core_sem tge (CMin_State fn a k (Vptr sp Int.zero) te) tm
-                                    (CMin_State fn s k (Vptr sp Int.zero) te) tm' /\
-    Mem.inject f' m' tm' /\
-    match_callstack prog f' m' tm' (Frame cenv tf e lenv te sp lo hi :: cs) (Mem.nextblock m') (Mem.nextblock tm') /\
-    inject_incr f f'  /\
-(******* The following five conditions are new -- but actually, only conditions 3-5 or used below*****)
-    Events.mem_unchanged_on (Events.loc_unmapped f) m m' /\
-    Events.mem_unchanged_on (Events.loc_out_of_reach f m) tm tm' /\
-    Events.inject_separated f f' m tm  /\
-    (forall b, Mem.valid_block m b -> Mem.valid_block m' b) (* actually <-> holds*)
-  /\ (forall b, Mem.valid_block tm b -> Mem.valid_block tm' b). 
-Proof.
-  intros until k. 
-  intros VS MCS VINJ MINJ KIND MEMCPY VAL.
-  assert (MV: match_var prog f id e m te sp cenv!!id).
-    inv MCS. inv MENV. auto.
-  inv MV; try congruence. rewrite KIND in H0; inv H0.
-  (* var_stack_array *)
-  unfold var_set_self in VS. rewrite <- H in VS. inv VS.
-  exploit match_callstack_match_globalenvs; eauto. intros [hi' MG].
-  assert (Events.external_call (EF_memcpy sz0 (Zmin al0 4)) ge (Vptr b0 Int.zero :: v :: nil) m Events.E0 Vundef m').
-    assumption.
-  exploit Events.external_call_mem_inject; eauto. 
-  eapply inj_preserves_globals; eauto.
-  intros [f' [vres' [tm' [EC' [VINJ' [MINJ' [UNMAPPED [OUTOFREACH [INCR SEPARATED]]]]]]]]].
-  exists f'; exists tm'.
-  split. eapply corestep_star_trans.
-           eapply corestep_star_one. eapply CompCertStep_CMin_corestep'. constructor. reflexivity. 
-         simpl.
-         eapply corestep_star_trans.
-           eapply corestep_star_one. eapply CompCertStep_CMin_corestep'. econstructor; eauto. 
-                constructor. apply make_stackaddr_correct. constructor. constructor. eauto. constructor.
-                  eapply Events.external_call_symbols_preserved_2; eauto.
-                  apply symbols_preserved. assumption.
-                  apply var_info_translated. assumption.
-                  apply var_info_rev_translated. assumption.
-               reflexivity.
-         simpl. eapply corestep_star_one. eapply CompCertStep_CMin_corestep. constructor. reflexivity.
-  split. auto.
-  split. apply match_callstack_incr_bound with (Mem.nextblock m) (Mem.nextblock tm).
-  eapply match_callstack_external_call; eauto.
-  intros. eapply Events.external_call_max_perm; eauto.
-  omega. omega.
-  eapply external_call_nextblock_incr; eauto.
-  eapply external_call_nextblock_incr; eauto.
-split.  auto.
-split; trivial.
-split; trivial.
-split; trivial.
-split; intros. inv MEMCPY. eapply Mem.storebytes_valid_block_1; eauto.
-   (*    apply prop_ext; split; intros. eapply Mem.storebytes_valid_block_1; eauto. eapply Mem.storebytes_valid_block_2; eauto.      *)
-eapply Events.external_call_valid_block; eauto. 
-Qed.
-
-(*Lemma appears to be new*)
-Lemma bind_parameters_validblock_2:
-forall gee e params vals m1 m2 (BP: bind_parameters gee e m1 params vals m2)
-b (B1:Mem.valid_block m2 b), Mem.valid_block m1 b.
-Proof. intros gee e params.
-  induction params; intros.
-   inv BP. trivial.
-  destruct vals; inv BP.
-    (*skalar*)
-      eapply Mem.store_valid_block_2. apply H8.
-      eapply (IHparams _ _ _ H9 _ B1). 
-    (*array*)
-      inv H7.
-      eapply Mem.storebytes_valid_block_2. apply H13.
-      eapply (IHparams _ _ _ H8 _ B1). 
-Qed.
-
-(*Lemma appears to be new, but was not needed after all in new proof*)
-Lemma bind_parameters_validblock_1:
-forall gee e params vals m1 m2 (BP: bind_parameters gee e m1 params vals m2)
-b (B1:Mem.valid_block m1 b), Mem.valid_block m2 b.
-Proof. intros gee e params.
-  induction params; intros.
-   inv BP. trivial.
-  destruct vals; inv BP.
-    (*skalar*)
-      eapply (IHparams _ _ _ H9). clear IHparams H9.
-      eapply Mem.store_valid_block_1; eauto.
-    (*array*)
-      eapply (IHparams _ _ _ H8). clear IHparams H8.
-      inv H7. 
-      eapply Mem.storebytes_valid_block_1; eauto.
-Qed.
-
-(*Lemma appears to be new, but was not needed after all in new proof*)
-Lemma bind_parameters_inject_separated_skalar:
-forall gee e params vals m1 m2 f' tm3 j tm1 m tm2 v b ch
-(CH: Mem.store ch m b 0 v = Some m1)
-(BP: bind_parameters gee e m1 params vals m2)
-(MINJ : Mem.inject f' m2 tm3)
-(SEP : Events.inject_separated j f' m1 tm2),
-Events.inject_separated j f' m tm1.
-Proof. intros.
-  intros bb; intros.
-     unfold Events.inject_separated in SEP.
-     destruct (SEP _ _ _ H H0).
-     split; intros XX.  
-       apply H1. eapply Mem.store_valid_block_1; eauto.
-     assert (~ Mem.valid_block m2 bb).
-       intros ZZ. apply H1. apply (bind_parameters_validblock_2 _ _ _ _ _ _ BP _ ZZ). 
-       unfold Mem.inject in MINJ. destruct MINJ.
-         rewrite (mi_freeblocks _ H3) in H0. inv H0.    
-Qed.
-
-(*Lemma appears to be new, but was not needed after all in new proof*)
-Lemma bind_parameters_inject_separated_array:
-forall gee e params vals m1 m2  m cpvals t n sz
-(MemCPY: Events.extcall_memcpy_sem sz n gee cpvals m t Vundef m1)
-(BP: bind_parameters gee e m1 params vals m2) 
-j' tm3 j tm1 tm2 
-(MINJ : Mem.inject j' m2 tm3)
-(SEP : Events.inject_separated j j' m1 tm2),
-Events.inject_separated j j' m tm1.
-Proof. intros. inv MemCPY.
-  intros bb; intros.
-     unfold Events.inject_separated in SEP.
-     destruct (SEP _ _ _ H7 H8).
-     split; intros XX.  
-       apply H9. eapply Mem.storebytes_valid_block_1; eauto.
-     assert (~ Mem.valid_block m2 bb).
-       intros ZZ. apply H9.  apply (bind_parameters_validblock_2 _ _ _ _ _ _ BP _ ZZ). 
-       unfold Mem.inject in MINJ. destruct MINJ.
-         rewrite (mi_freeblocks _ H11) in H8. inv H8.    
-Qed.
-
-Lemma MS_store_parameters_correct:
-  forall e lenv te m1 params vl m2,
-  bind_parameters ge e m1 params vl m2 ->
-  forall s j1 cenv tf sp lo hi cs tm1 fn' k,
-  vars_vals_match j1 params vl te ->
-  list_norepet (List.map variable_name params) ->
-  Mem.inject j1 m1 tm1 ->
-  match_callstack prog j1 m1 tm1 (Frame cenv tf e lenv te sp lo hi :: cs) (Mem.nextblock m1) (Mem.nextblock tm1) ->
-  store_parameters cenv params = OK s ->
- exists j2, exists tm2,
-     corestep_star CMin_core_sem tge (CMin_State fn' s k (Vptr sp Int.zero) te) tm1
-                 (CMin_State fn' Sskip k (Vptr sp Int.zero) te) tm2
-  /\ Mem.inject j2 m2 tm2
-  /\ match_callstack prog j2 m2 tm2 (Frame cenv tf e lenv te sp lo hi :: cs) (Mem.nextblock m2) (Mem.nextblock tm2)
-  /\ inject_incr j1 j2
-(********* The following 3 conditions are new*****)
-  /\ Events.inject_separated j1 j2 m1 tm1
-  /\ (forall b, Mem.valid_block m1 b -> Mem.valid_block m2 b)
-  /\ (forall b, Mem.valid_block tm1 b -> Mem.valid_block tm2 b).
-Proof.
-  induction 1.
-  (* base case *)
-  intros; simpl. monadInv H3. rename m into m1.
-  exists j1. exists tm1. split. eapply corestep_star_zero.
-       split; trivial.
-       split; trivial.
-       split; trivial.
-       split. apply inject_separated_same_meminj.
-       split; trivial.
-  (* scalar case *)
-  rename m1 into mm1. rename m into m1.
-  intros until k.  intros VVM NOREPET MINJ MATCH STOREP.
-  monadInv STOREP. inv VVM. inv NOREPET. 
-  exploit MS_var_set_self_correct_scalar; eauto.
-    econstructor; eauto. econstructor; eauto.
-  intros [tmm1 [EXEC1 [MINJ1 [MATCH1 [VB TVB]]]]]. 
-  exploit IHbind_parameters; eauto.
-  intros [j2 [tm2 [EXEC2 [MINJ2 [MATCH2 [INJ2 [SEP2 [VB2 TVB2]]]]]]]]. 
-  exists j2; exists tm2.
-  split. eapply corestep_star_trans; eauto.
-  split; trivial.
-  split; trivial.
-  split; trivial.
-  split.
-      intros bb; intros. destruct (SEP2 _ _ _ H3 H4).
-      split; intros N. (*rewrite VB in N. apply (H7 N).*) apply H7. apply (VB _ N).
-                                (*rewrite TVB in N. apply (H9 N). *) apply H9. apply (TVB _ N).
-  split; intros.   (*rewrite VB. apply VB2. *) apply VB2. apply (VB _ H3).
-           apply TVB2. (*rewrite <- TVB. assumption. *) apply (TVB _ H3).
-  (* array case *)
-  intros until k.  intros VVM NOREPET MINJ MATCH STOREP.
-  monadInv STOREP. inv VVM. inv NOREPET.
-  exploit MS_var_set_self_correct_array; eauto.
-  intros [f2 [tm2 [EXEC1 [MINJ1 [MATCH1 [INCR1 [UcOn [TUcOn1 [SEP1 [VB1 TVB1]]]]]]]]]].
-  clear UcOn TUcOn1. (*this shows that the first 2 new conditions of MS_var_set_self_correct_array are in fact superfluous*)
-  exploit IHbind_parameters. eapply vars_vals_match_incr; eauto. auto. eauto. eauto. eauto. 
-  intros [f3 [tm3 [EXEC2 [MINJ2 [MATCH2 [INCR2 [SEP2 [VB2 TVB2]]]]]]]]. 
-  exists f3; exists tm3.
-  split. eapply corestep_star_trans; eauto.
-  split. auto. split. auto. 
-  split. eapply inject_incr_trans; eauto.
-  split. clear EXEC2 MATCH2 EXEC1 MATCH1 IHbind_parameters.
-     intros bb; intros.
-       remember (f2 bb) as z; destruct z; apply eq_sym in Heqz.
-       (*Some p*) destruct p.
-             assert (f3 bb = Some (b0, z)). apply INCR2 in Heqz. assumption.
-             rewrite H6 in H3. inv H3.
-             eapply SEP1. assumption. eassumption.
-       (*None*) 
-             destruct (SEP2 _ _ _ Heqz H3).
-             split; intros N. (*rewrite VB1 in N. apply (H6 N).*) apply H6. apply (VB1 _ N).
-                 apply TVB1 in N. apply (H7 N).
-  split; intros. (*rewrite VB1. apply VB2.*) apply VB2. apply (VB1 _ H2).
-           apply TVB2. apply (TVB1 _ H2).
-Qed. 
-
-(***** All the additional conditions in the above auxiliary lemmas were needed for proving
- the condition Events.inject_separated j j' m tmt in his lemma; otherwise, the claim is as before, 
-  just updated by replacing star step by corestep_star, as ususal*)
-Lemma MS_function_entry_ok:
-  forall tf fn m e m1 vargs m2 j cs tm cenv tm1 sp tvargs s fn' k,
-  list_norepet (fn_params_names fn ++ fn_vars_names fn) ->
-  alloc_variables empty_env m (fn_variables fn) e m1 ->
-  bind_parameters ge e m1 fn.(Csharpminor.fn_params) vargs m2 ->
-  match_callstack prog j m tm cs (Mem.nextblock m) (Mem.nextblock tm) ->
-  build_compilenv gce fn = (cenv, tf.(fn_stackspace)) ->
-  tf.(fn_stackspace) <= Int.max_unsigned ->
-  Mem.alloc tm 0 tf.(fn_stackspace) = (tm1, sp) ->
-  let tparams := List.map for_var (fn_params_names fn) in
-  let tvars := List.map for_var (fn_vars_names fn) in
-  let ttemps := List.map for_temp (Csharpminor.fn_temps fn) in
-  let te := set_locals (tvars ++ ttemps) (set_params tvargs tparams) in
-  val_list_inject j vargs tvargs ->
-  Mem.inject j m tm ->
-  store_parameters cenv fn.(Csharpminor.fn_params) = OK s ->
-  exists j', exists tm2,
-     corestep_star CMin_core_sem tge (CMin_State fn' s k (Vptr sp Int.zero) te) tm1
-                                 (CMin_State fn' Sskip k (Vptr sp Int.zero) te) tm2
-  /\ Mem.inject j' m2 tm2
-  /\ inject_incr j j'
-
-  (*This condition is new*)
-  /\ Events.inject_separated j j' m tm
-
-  /\ match_callstack prog j' m2 tm2
-       (Frame cenv tf e empty_temp_env te sp (Mem.nextblock m) (Mem.nextblock m1) :: cs)
-       (Mem.nextblock m2) (Mem.nextblock tm2).
-Proof.
-  intros.
-  exploit MS_match_callstack_alloc_variables; eauto.
-  intros [j1 [INCR1 [MINJ1 [MATCH1 [VB1 [SP1 SEP1]]]]]].
-  exploit vars_vals_match_holds.
-    eexact H. 
-    apply val_list_inject_incr with j. eauto. eauto.
-    eapply bind_parameters_normalized; eauto.
-  instantiate (1 := Csharpminor.fn_temps fn). 
-  fold tvars. fold ttemps. fold (fn_params_names fn). fold tparams. fold te.   
-  intro VVM.
-  exploit MS_store_parameters_correct.
-    eauto. eauto. eauto. eapply list_norepet_append_left; eauto.
-    eexact MINJ1. eexact MATCH1. eauto.
-  intros [j2 [tm2 [EXEC [MINJ2 [MATCH2 [INCR2 [SEP2 [VB2 TVB2]]]]]]]].
-  exists j2; exists tm2. 
-  split; eauto. split; auto. split; auto. eapply inject_incr_trans; eauto.
-Qed.
-
-Lemma MS_step_case_InternalCall:
-forall cenv  f j m tm e cs k tk vargs targs x m1 m2
-(Param: list_norepet (fn_params_names f ++ fn_vars_names f))
-(AllocVars : alloc_variables empty_env m (fn_variables f) e m1)
-(BindParams : bind_parameters ge e m1 (Csharpminor.fn_params f) vargs m2)
-(MINJ : Mem.inject j m tm)
-(MCS : match_callstack prog j m tm cs (Mem.nextblock m) (Mem.nextblock tm))
-(MK : match_cont k tk (fn_return f) cenv nil cs)
-(ISCC: Csharpminor.is_call_cont k)
-(ARGSINJ : val_list_inject j vargs targs)
-(EQ : transl_function gce f = OK x),
-exists c2' : CMin_core,
-  exists m2' : mem,
-       corestep_plus CMin_core_sem tge (CMin_Callstate (AST.Internal x) targs tk) tm c2' m2' /\
-  exists j' : meminj,
-        inject_incr j j' /\
-        (*again, have inject-sparatated here, as per definition of match relation*) 
-         Events.inject_separated j j' m tm /\
-  exists c',
-        inj_match_states_star unit match_cores MC_measure (tt,c') j'
-           (CSharpMin_State f (Csharpminor.fn_body f) k e empty_temp_env) m2 c2' m2'.
-Proof. intros.
-  generalize EQ; clear EQ; unfold transl_function.
-  caseEq (build_compilenv gce f). intros ce sz BC.
-  destruct (zlenv sz Int.max_unsigned); try congruence.
-  intro TRBODY.
-  generalize TRBODY; intro TMP. monadInv TMP.
-  set (tf := mkfunction (Csharpminor.fn_sig f) 
-                        (List.map for_var (fn_params_names f))
-                        (List.map for_var (fn_vars_names f)
-                         ++ List.map for_temp (Csharpminor.fn_temps f))
-                        sz
-                        (Sseq x1 x0)) in *.
-  caseEq (Mem.alloc tm 0 (fn_stackspace tf)). intros tm' sp ALLOC'.
-  exploit MS_function_entry_ok; eauto; simpl; auto.  
-  intros [j' [tm2 [EXEC [MINJ2 [IINCR [SEP2 MCS2]]]]]].
-  eexists; eexists; split.
-    eapply corestep_plus_star_trans.
-      eapply corestep_plus_one. eapply CompCertStep_CMin_corestep'. constructor; simpl; eauto. reflexivity.  
-    simpl.
-    eapply corestep_star_trans.
-      eapply corestep_star_one. eapply CompCertStep_CMin_corestep'. constructor. reflexivity.
-    simpl.
-    eapply corestep_star_trans. apply EXEC.
-      simpl. eapply corestep_star_one. eapply CompCertStep_CMin_corestep'. constructor. reflexivity.
-  simpl in *.
-  exists j'. split. assumption.
-  split. assumption.
-  exists (CSharpMin_State f(Csharpminor.fn_body f) k e empty_temp_env).
-  left.
-  econstructor. eexact TRBODY. eauto. eexact MINJ2. 
-  eexact MCS2.
-  inv MK; simpl in ISCC; contradiction || econstructor; eauto.
-Qed.
-
-(******************End of updated section for internal call rule*****************************)
-(************************************************************************************)
-
-Lemma MS_step_case_Return:
-forall j m tm cs f e lenv k tk ty cenv v tv optid
-(MINJ : Mem.inject j m tm)
-(MCS : match_callstack prog j m tm cs (Mem.nextblock m) (Mem.nextblock tm))
-(MK : match_cont (Csharpminor.Kcall optid f e lenv k) tk ty cenv nil cs)
-(RESINJ : val_inject j v tv),
-exists c2' : CMin_core,
-  exists m2' : mem,
-       corestep_plus CMin_core_sem tge (CMin_Returnstate tv tk) tm c2' m2'  /\
-    exists c', 
-       inj_match_states_star unit match_cores MC_measure (tt,c') j
-             (CSharpMin_State f Csharpminor.Sskip k e (set_optvar optid v lenv)) m c2' m2' .
-Proof. intros.
-  inv MK. simpl.
-  eexists; eexists; split.
-       eapply corestep_plus_one. eapply CompCertStep_CMin_corestep'. econstructor; eauto. reflexivity.
-  simpl.
-  exists  (CSharpMin_State f Csharpminor.Sskip k e (set_optvar optid v lenv)).
-    left. unfold set_optvar. destruct optid; simpl option_map; econstructor; eauto.              
-         eapply match_callstack_set_temp; eauto. 
-Qed. 
-
-Lemma MS_step: forall (c1 : CSharpMin_core) (m1 : mem) (c1' : CSharpMin_core) (m1' : mem),
-corestep CSharpMin_CompcertCoreSem ge c1 m1 c1' m1' ->
-forall (dc : inj_star_data core_data) (c2 : CMin_core) (j : meminj)
-  (m2 : mem),
-inj_match_states_star core_data match_cores MC_measure dc j c1 m1 c2 m2 ->
-exists c2' : CMin_core,
-  exists m2' : mem,
-    exists dc' : inj_star_data core_data,
-      exists j' : meminj,
-        inject_incr j j' /\
-        Events.inject_separated j j' m1 m2 /\
-        inj_match_states_star core_data match_cores MC_measure dc' j' c1' m1'
-          c2' m2' /\
-        (corestep_plus CMin_CompcertCoreSem tge c2 m2 c2' m2' \/
-         corestep_star CMin_CompcertCoreSem tge c2 m2 c2' m2' /\
-         inj_star_ord core_data MC_order MC_measure dc' dc).
-Proof.
-  intros. destruct dc as [DATA CORE]. subst. unfold core_data in *. destruct DATA.
-   destruct (CSharpMin_corestep_2_CompCertStep _ _ _ _ _ H) as [t Ht]. simpl in *.
-  apply CSharpMin_corestep_not_at_external in H.
-destruct H0.
-   apply MC_MSI in H0. rename H0 into MSTATE.
-   inv Ht; simpl in *.
-  (*skip seq*)
-      destruct c1; simpl in *; try inv H1. 
-      destruct c1'; simpl in *; try inv H3. simpl in *. 
-      inv MSTATE; simpl in *. 
-      monadInv TR.
-      destruct c2; simpl in *; try inv H8. 
-      destruct (MS_step_case_SkipSeq _ _ _ _ _ _ _ _ _ _ _ _ _ _ _ _ _ _ TRF MINJ MK MCS) as [c2' [m2' [cstepPlus [c' MS]]]].
-      exists c2'. exists m2'. exists (tt,c'). exists j.
-      split. apply inject_incr_refl.
-      split. apply inject_separated_same_meminj.
-      auto.
-  (*skip Block*)
-      destruct c1; simpl in *; try inv H1. 
-      destruct c1'; simpl in *; try inv H3. 
-      inv MSTATE; simpl in *. 
-      monadInv TR.
-      destruct c2; simpl in *; try inv H8. 
-      destruct (MS_step_case_SkipBlock _ _ _ _ _ _ _ _ _ _ _ _ _ _ _ _ _ TRF MINJ MK MCS) as [c2' [m2' [cstepPlus [c' MS]]]].
-      exists c2'. exists m2'. exists (tt,c'). exists j.
-      split. apply inject_incr_refl.
-      split. apply inject_separated_same_meminj.
-      auto.
-  (*skip Call*)
-      destruct c1; simpl in *; try inv H0. 
-      destruct c1'; simpl in *; try inv H1. 
-      inv MSTATE; simpl in *. 
-      monadInv TR.
-      destruct c2; simpl in *; try inv H11.
-      destruct (MS_step_case_SkipCall  _ _ _ _ _ _ _ _ _ _ _ _ _ _ _ _ _ _ H2 H3 H5 TRF MINJ MK MCS) as [c2' [m2' [cstepPlus [c' MS]]]].
-      exists c2'. exists m2'. exists (tt,c'). exists j.
-      split. apply inject_incr_refl.
-      split. apply inject_separated_same_meminj.
-      auto.
-   (*assign*)
-      destruct c1; simpl in *; try inv H0. 
-      destruct c1'; simpl in *; try inv H1. 
-      inv MSTATE; simpl in *.
-      monadInv TR.
-      destruct c2; simpl in *; try inv H10.
-      rename  m1' into m'. rename m1 into m. rename m2 into tm. rename k0 into tk. rename f0 into tfn. rename e0 into te.
-      destruct (MS_step_case_Assign  _ _ _ _ _ _ _ _ _ _ _ _ _ _ _ _ _ _ _ _ _ _ _ _ H2 H4 TRF MINJ MK MCS EQ EQ0) as [c2' [m2' [cstepPlus [c' MS]]]].
-      exists c2'. exists m2'. exists (tt,c'). exists j.
-      split. apply inject_incr_refl.
-      split. apply inject_separated_same_meminj.
-      auto.
-   (*set*)
-      destruct c1; simpl in *; try inv H0. 
-      destruct c1'; simpl in *; try inv H1. 
-      inv MSTATE; simpl in *.
-      monadInv TR.
-      destruct c2; simpl in *; try inv H9.
-      destruct (MS_step_case_Set _ _ _ _ _ _ _ _ _ _ _ _ _ _ _ _ _ _ _ _ _ id H3 TRF MINJ MCS MK EQ) as [c2' [m2' [cstepPlus [c' MS]]]].
-      exists c2'. exists m2'. exists (tt,c'). exists j.
-      split. apply inject_incr_refl.
-      split. apply inject_separated_same_meminj.
-      auto.
-   (*store*)
-      destruct c1; simpl in *; try inv H0. 
-      destruct c1'; simpl in *; try inv H1. 
-      inv MSTATE; simpl in *.
-      monadInv TR.
-      destruct c2; simpl in *; try inv H11. rename f0 into tfn. rename m1 into m. rename m2  into tm. rename e0 into te. rename k0 into tk. rename  m1' into m'.
-      destruct (MS_step_case_Store _ _ _ _ _ _ _ _ _ _ _ _ _ _ _ _ _ _ _ _ _ _ _ _ _ _ _ H5 H2 H3 TRF MINJ MCS MK EQ EQ1) as [c2' [m2' [cstepPlus [c' MS]]]].
-      exists c2'. exists m2'. exists (tt,c'). exists j.
-      split. apply inject_incr_refl.
-      split. apply inject_separated_same_meminj.
-      auto.
-   (*call*)
-      destruct c1; simpl in *; try inv H0. 
-      destruct c1'; simpl in *; try inv H1. 
-      inv MSTATE; simpl in *.
-      monadInv TR.
-      destruct c2; simpl in *; try inv H11. 
-      rename f into fd. rename f0 into f. rename f1 into tfn.
-      rename m1' into m. rename m2  into tm. rename e into te.
-      rename e0 into e.  rename k0 into tk. rename  le0 into le.
-      destruct (MS_step_case_Call _ _ _ _ _ _ _ _ _ _ _ _ _ _ _ _ _ _ _ _ _ _ _ optid _ _ H2 H3 H4 TRF MINJ MCS MK EQ EQ1) as [c2' [m2' [cstepPlus [c' MS]]]].
-      exists c2'. exists m2'. exists (tt,c'). exists j.
-      split. apply inject_incr_refl.
-      split. apply inject_separated_same_meminj.
-      auto.
-   (*builtin*)
-      destruct c1; simpl in *; try inv H0. 
-      destruct c1'; simpl in *; try inv H1. 
-      inv MSTATE; simpl in *.
-      monadInv TR.
-      destruct c2; simpl in *; try inv H10. 
-      rename f0 into tfn. 
-      rename m1 into m. rename m2  into tm. rename e into te.
-      rename e0 into e.  rename k0 into tk. rename  le0 into le.  rename m1' into m'.
-      destruct (MS_step_case_Builtin _ _ _ _ _ _ _ _ _ _ _ _ _ _ _ _ _ _ _ _ optid _ _ _ _ H2 H4 TRF MINJ MCS MK EQ) as [c2' [m2' [cstepPlus [j' [InjIncr [InjSep [c' MS]]]]]]].
-      exists c2'. exists m2'. exists (tt,c'). exists j'. auto.
-  (* seq *)
-      destruct c1; simpl in *; try inv H1. 
-      destruct c1'; simpl in *; try inv H3. 
-     rename k0 into k.
-      inv MSTATE. 
-      (*Case 1*) 
-         monadInv TR.
-         destruct c2; simpl in *; try inv H8.
-         rename f0 into tfn. rename e0 into te. rename k0 into tk.
-         exists  (CMin_State tfn x (Kseq x0 tk) (Vptr sp Int.zero) te). exists m2. 
-         exists (tt,CSharpMin_State f s (Csharpminor.Kseq s2 k) e lenv).
-         exists j. 
-                split. apply inject_incr_refl.
-                split. apply inject_separated_same_meminj.
-                split; left; simpl. 
-                     econstructor; eauto.
-                          econstructor; eauto.
-                     apply corestep_plus_one. eapply CompCertStep_CMin_corestep.  econstructor. reflexivity.
-       (* seq 2 *)
-          exists c2. exists m2. exists (tt,CSharpMin_State f s (Csharpminor.Kseq s2 k) e lenv). exists j.
-                split. apply inject_incr_refl.
-                split. apply inject_separated_same_meminj. 
-                destruct  c2; simpl in *; inv H9.
-                split.  left. econstructor; try eassumption.
-                   right. split. apply corestep_star_zero.
-simpl. eapply lex_ord_right. simpl. unfold ltof. (*unfold MC_measure. simpl. *) admit. (*CORE is unconstrained!?*)
-(* ifthenelse *)
-      destruct c1; simpl in *; try inv H0. 
-      destruct c1'; simpl in *; try inv H1. 
-      inv MSTATE. 
-      monadInv TR.
-      destruct c2; simpl in *; try inv H10. 
-         rename f0 into tfn. rename e0 into te. rename k0 into tk.
-      rename m1' into m. rename m2  into tm. 
-      destruct (MS_step_case_Ite _ _ _ _ _ _ _ _ _ _ _ _ _ _ _ _ _ _ _ _ _ _ _ _ _ _ H2 H4 TRF MINJ MCS MK EQ EQ1 EQ0) as [c2' [m2' [cstepPlus [c' MS]]]].
-      exists c2'. exists m2'. exists (tt,c'). exists j.
-      split. apply inject_incr_refl.
-      split. apply inject_separated_same_meminj.
-      auto.
-  (*loop*)
-      destruct c1; simpl in *; try inv H1. 
-      destruct c1'; simpl in *; try inv H3. 
-      inv MSTATE. 
-      monadInv TR.
-      destruct c2; simpl in *; try inv H8. 
-         rename f0 into tfn. rename e0 into te. rename k0 into tk.
-      rename m1' into m. rename m2  into tm. 
-      destruct (MS_step_case_Loop _ _ _ _ _ _ _ _ _ _ _ _ _ _ _ _ _ _ _ TRF MINJ MCS MK EQ) as [c2' [m2' [cstepPlus [c' MS]]]].
-      exists c2'. exists m2'. exists (tt,c'). exists j.
-      split. apply inject_incr_refl.
-      split. apply inject_separated_same_meminj.
-      auto.
-  (*block*)
-      destruct c1; simpl in *; try inv H1. 
-      destruct c1'; simpl in *; try inv H3. 
-      inv MSTATE. 
-      monadInv TR.
-      destruct c2; simpl in *; try inv H8. 
-         rename f0 into tfn. rename e0 into te. rename k0 into tk.
-      rename m1' into m. rename m2  into tm.  rename s0 into s.
-      destruct (MS_step_case_Block _ _ _ _ _ _ _ _ _ _ _ _ _ _ _ _ _ _ _ TRF MINJ MCS MK EQ) as [c2' [m2' [cstepPlus [c' MS]]]].
-      exists c2'. exists m2'. exists (tt,c'). exists j.
-      split. apply inject_incr_refl.
-      split. apply inject_separated_same_meminj.
-      auto.
-  (*exit seq*)
-      destruct c1; simpl in *; try inv H1. 
-      destruct c1'; simpl in *; try inv H3. 
-      inv MSTATE. 
-      monadInv TR.
-      destruct c2; simpl in *; try inv H8. 
-         rename f0 into tfn. rename e0 into te. rename k0 into tk.
-      rename m1' into m. rename m2  into tm.
-      destruct (MS_step_case_ExitSeq _ _ _ _ _ _ _ _ _ _ _ _ _ _ _ _ _ n _ TRF MINJ MCS MK) as [c2' [m2' [cstepPlus [c' MS]]]].
-      exists c2'. exists m2'. exists (tt,c'). exists j.
-      split. apply inject_incr_refl.
-      split. apply inject_separated_same_meminj.
-      auto.
-  (*exit block 0*)
-      destruct c1; simpl in *; try inv H1. 
-      destruct c1'; simpl in *; try inv H3. 
-      inv MSTATE. 
-      monadInv TR.
-      destruct c2; simpl in *; try inv H8. 
-         rename f0 into tfn. rename e0 into te. rename k0 into tk.
-      rename m1' into m. rename m2  into tm.
-      destruct (MS_step_case_ExitBlockZero _ _ _ _ _ _ _ _ _ _ _ _ _ _ _ _ _ TRF MINJ MCS MK) as [c2' [m2' [cstepPlus [c' MS]]]].
-      exists c2'. exists m2'. exists (tt,c'). exists j.
-      split. apply inject_incr_refl.
-      split. apply inject_separated_same_meminj.
-      auto.
-  (*exit block n+1*)
-      destruct c1; simpl in *; try inv H1. 
-      destruct c1'; simpl in *; try inv H3. 
-      inv MSTATE. 
-      monadInv TR.
-      destruct c2; simpl in *; try inv H8. 
-         rename f0 into tfn. rename e0 into te. rename k0 into tk.
-      rename m1' into m. rename m2  into tm.
-      destruct (MS_step_case_ExitBlockNonzero _ _ _ _ _ _ _ _ _ _ _ _ _ _ _ _ _ n TRF MINJ MCS MK) as [c2' [m2' [cstepPlus [c' MS]]]].
-      exists c2'. exists m2'. exists (tt,c'). exists j.
-      split. apply inject_incr_refl.
-      split. apply inject_separated_same_meminj.
-      auto.
-  (*switch*)
-      destruct c1; simpl in *; try inv H0. 
-      destruct c1'; simpl in *; try inv H1. 
-      inv MSTATE. 
-      monadInv TR.
-      destruct c2; simpl in *; try inv H9. 
-         rename f0 into tfn.  rename e0 into te.
-         rename k0 into tk. rename m1' into m. rename m2  into tm.  rename s into ts.
-      destruct (MS_step_case_Switch _ _ _ _ _ _ _ _ _ _ _ _ _ _ _ _ _ _ _ _ _ _ _ H3 TRF MINJ MCS MK EQ EQ0) as [c2' [m2' [cstepPlus [c' MS]]]].
-      exists c2'. exists m2'. exists (tt,c'). exists j.
-      split. apply inject_incr_refl.
-      split. apply inject_separated_same_meminj.
-      auto.
-  (*return none*)
-      destruct c1; simpl in *; try inv H0. 
-      destruct c1'; simpl in *; try inv H1. 
-      inv MSTATE. 
-      monadInv TR.
-      destruct c2; simpl in *; try inv H9. 
-       rename f into tfn.  rename f0 into f. rename e into te. rename e0 into e.
-         rename k0 into tk. rename m1 into m. rename m2  into tm. rename m1'  into m'.  rename le0 into le.
-      destruct (MS_step_case_ReturnNone _ _ _ _ _ _ _ _ _ _ _ _ _ _ _ _ _ _ H3 TRF MINJ MCS MK) as [c2' [m2' [cstepPlus [c' MS]]]].
-      exists c2'. exists m2'. exists (tt,c'). exists j.
-      split. apply inject_incr_refl.
-      split. apply inject_separated_same_meminj.
-      auto.
-  (*return some*)
-      destruct c1; simpl in *; try inv H0. 
-      destruct c1'; simpl in *; try inv H1. 
-      inv MSTATE. 
-      monadInv TR.
-      destruct c2; simpl in *; try inv H10. 
-       rename f into tfn.  rename f0 into f. rename e into te. rename e0 into e. rename k into tk.
-         rename k0 into k. rename m1 into m. rename m2  into tm. rename m1'  into m'.  rename le0 into le. rename v0 into v.
-      destruct (MS_step_case_ReturnSome _ _ _ _ _ _ _ _ _ _ _ _ _ _ _ _ _ _ _ _ _ _ H2 H4 TRF MINJ MCS MK EQ) as [c2' [m2' [cstepPlus [c' MS]]]].
-      exists c2'. exists m2'. exists (tt,c'). exists j.
-      split. apply inject_incr_refl.
-      split. apply inject_separated_same_meminj.
-      auto.
-  (*label*)
-      destruct c1; simpl in *; try inv H1. 
-      destruct c1'; simpl in *; try inv H3. 
-      inv MSTATE. 
-      monadInv TR.
-      destruct c2; simpl in *; try inv H8. 
-       rename f0 into tfn. rename e0 into te. 
-         rename k0 into tk. rename m1' into m. rename m2  into tm. rename s0 into s.  
-      destruct (MS_step_case_Label _ _ _ _ _ _ _ _ _ _ _ _ _ _ _ _ _ lbl _ _ TRF MINJ MCS MK EQ) as [c2' [m2' [cstepPlus [c' MS]]]].
-      exists c2'. exists m2'. exists (tt,c'). exists j.
-      split. apply inject_incr_refl.
-      split. apply inject_separated_same_meminj.
-      auto.
-  (*goto*)
-      destruct c1; simpl in *; try inv H0. 
-      destruct c1'; simpl in *; try inv H1. 
-      inv MSTATE. 
-      monadInv TR.
-      destruct c2; simpl in *; try inv H9. 
-       rename f0 into tfn. rename e0 into te. 
-         rename k1 into tk. rename s into s'.  rename k into k'. rename k0 into k. rename m1' into m. rename m2  into tm.
-      destruct (MS_step_case_Goto _ _ _ _ _ _ _ _ _ _ _ _ _ _ _ _ _ _ _ _ H3 TRF MINJ MCS MK) as [c2' [m2' [cstepPlus [c' MS]]]].
-      exists c2'. exists m2'. exists (tt,c'). exists j.
-      split. apply inject_incr_refl.
-      split. apply inject_separated_same_meminj.
-      auto.
-(* internal call *)
-      destruct c1; simpl in *; try inv H0. 
-      destruct c1'; simpl in *; try inv H1. 
-      inv MSTATE. 
-      monadInv TR.
-      destruct c2; simpl in *; try inv H9. 
-      rename m1 into m. rename m2 into tm. rename f0 into f. rename e0 into e.
-      rename m0 into m1. rename args into vargs. rename m1' into m2.
-      rename k0 into tk. rename args0 into targs. 
-      destruct (MS_step_case_InternalCall _ _ _ _ _ _ _ _ _ _ _ _ _ _ H2 H3 H5 MINJ MCS MK ISCC ARGSINJ EQ) as [c2' [m2' [cstepPlus [j' [InjIncr [InjSep [c' MS]]]]]]].
-      exists c2'. exists m2'. exists (tt,c'). exists j'. auto.
-(* external call *)
-      destruct c1; simpl in *; try inv H0. inv H. 
-   (*nothing to show here - cf corestep not at external *) 
- (*     destruct c1'; simpl in *; try inv H1. 
-      inv MSTATE. 
-      monadInv TR.
-      destruct c2; simpl in *; try inv H7.  
-      rename m1 into m. rename m2 into tm. 
-      rename k0 into tk. rename args0 into targs.  rename m1' into m'. 
-  inv MSTATE. monadInv TR. rename f into j.
-  destruct (transl_step_case_ExternalCall _ _ _ _ _ _ _ _ _ _ _ _ _ H MINJ MCS MK ISCC ARGSINJ) as [T2 [Steps [j' [Inc MSI]]]].
-   apply matchInj_Elim in MSI. eauto.*)
-
-(* return *)
-      destruct c1; simpl in *; try inv H1. 
-      destruct c1'; simpl in *; try inv H3. 
-      inv MSTATE. 
-      destruct c2; simpl in *; try inv H5. rename m1' into m. rename m2 into tm. rename f0 into f. rename e0 into e. rename k into tk. rename k0 into k. rename v into tv. rename v0 into v.
-      destruct (MS_step_case_Return _ _ _ _ _ _ _ _ _ _ _ _ tv optid MINJ MCS MK RESINJ) as [c2' [m2' [cstepPlus [c' MS]]]]. 
-      exists c2'. exists m2'. exists (tt,c'). exists j.
-      split. apply inject_incr_refl.
-      split. apply inject_separated_same_meminj.
-      auto.
-destruct H0. 
-Qed.
-       unfold core_data in *. destruct DATA.
-       eapply MC_matchstates in H0.
-       rewrite (MC_atExt _ _ _ _ H0) in H.
-       destruct (transl_step_correct _ _ TRANSL _ _ _ Ht _ H0) as [[T2 [SPlus X]] | X]. 
-           destruct (CompCertStepPlus_2_CMin_corestepPlus _ _ _ _ _ SPlus H) as [c2' [m2' [? CMinPlus]]]; subst.
-           apply MC_matchcores in X. destruct X as [j' Hj'].
-           exists c2'. exists m2'. exists (tt,CORE). exists j'.
-             split. admit. (*not satisfied - we actuall have to redo the proof of transl_step_correct for this reason! -- j/j' are hidden*)
-             split . admit. (*same here*)
-             split; left; assumption.
-        destruct X as [MEAS [X  MSP]]. subst. 
-           apply MC_matchcores in MSP. destruct MSP as [j' Hj'].
-           exists c2. exists m2. exists (tt,c1'). exists j'.
-             split. admit. (*not satisfied - we actuall have to redo the proof of transl_step_correct for this reason! -- j/j' are hidden*)
-             split . admit. (*same here*)
-             split. simpl. left; assumption.
-             right. split. exists O.  reflexivity. 
-             simpl. admit (*.. measure stuff . *).
-  destruct H0. 
-       unfold core_data in *. destruct DATA.
-       eapply MC_matchstates in H1.
-       rewrite (MC_atExt _ _ _ _ H1) in H.
-       destruct (transl_step_correct _ _ TRANSL _ _ _ Ht _ H0) as [[T2 [SPlus X]] | X]. 
-           destruct (CompCertStepPlus_2_CMin_corestepPlus _ _ _ _ _ SPlus H) as [c2' [m2' [? CMinPlus]]]; subst.
-           apply MC_matchcores in X. destruct X as [j' Hj'].
-           exists c2'. exists m2'. exists (tt,CORE). exists j'.
-             split. admit. (*not satisfied - we actuall have to redo the proof of transl_step_correct for this reason! -- j/j' are hidden*)
-             split . admit. (*same here*)
-             split; left; assumption.
-        destruct X as [MEAS [X  MSP]]. subst. 
-           apply MC_matchcores in MSP. destruct MSP as [j' Hj'].
-           exists c2. exists m2. exists (tt,c1'). exists j'.
-             split. admit. (*not satisfied - we actuall have to redo the proof of transl_step_correct for this reason! -- j/j' are hidden*)
-             split . admit. (*same here*)
-             split. simpl. left; assumption.
-             right. split. exists O.  reflexivity. 
-             simpl. admit (*.. measure stuff . *).
-      
-    unfold core_data in *. destruct X as [MEAS [TRACE MS]]. subst.
-      destruct (transl_step_correct _ _ TRANSL _ _ _ Ht _ H0) as [[T2 [SPlus X]] | X]. 
-      rewrite (MC_atExt _ _ _ _ H0) in H.
-      destruct (CompCertStepPlus_2_CMin_corestepPlus _ _ _ _ _ SPlus H) as [c2' [m2' [? CMinPlus]]]; subst.
-      apply MC_matchcores in X. destruct X as [j' Hj'].
-      exists c2'. exists m2'. exists (tt,CORE). exists j'.
-        split. admit. (*not satisfied - we actuall have to redo the proof of transl_step_correct for this reason! -- j/j' are hidden*)
-        split . admit. (*same here*)
-        split; left; assumption.
-         
-  
-        left. assumption.
- 
-        exis unfold inj_star_data. unit. exists tt. 
-       
- xx CompCertStepStar_2_corestepstar in SPlus.
-            admit.
-          destruct (CompCertStep_2_corestep _ _ _ _ _ Ht H) as [q' [m' [? MinStep]]]. clear Ht.
-          apply CSharpMin_core2state_injective in H1. destruct H1; subst.   (*We can't simply left Cminor_CompCertsemantics.CompCertStep_corestep
-                         to plus, since we have no guarantee that all intermediate steps in assumption X
-                         satisfy atExternal = None.
-                         I believe they do
-        simpl in X.
-   inv H0; simpl in *.
-     eapply MC_matchstates in MCS.
-    assert (ZZ:= MC_matchstates _ _ _ _ _ _ _ MCS).
-(*   destruct c1; destruct c1'. simpl in H.*)
-   destruct (corestep_CompCertStep ge (CSharpMin_State f s k e lenv) m1 (CSharpMin_State f0 s0 k0 e0 le0) m1' H) as [t Ht]. simpl in *.
-   assert (X:= transl_step_correct _ _ TRANSL _ _ _ Ht). simpl in X.
-   inv H0; simpl in *. Focus 2.
-   inv H. simpl in *.
-       inv H1. simpl in *.
-          destruct H0. simpl in H. exists c2. exists m2.   destruct H. inv H. 
-   generalize dependent dc. generalize dependent j.  generalize dependent m2.  generalize dependent c2.
-   (*State State*)  admit.
-   (*State CallState*)  admit.
-   (*State ReturnState*) admit.
-   (*Callstate State*) admit.
-   (*Returnstate*)
-        simpl in *. induction H. inv H.
-  unfold corestep  in H. simpl in *. unfold CSharpMin_corestep in H. inv H. induction H.  
-Admitted.
-
-
-Lemma Csharpminor_Cminor_sim_inj: forall entrypoints
-(*              ExternIdents  (ext_ok : CompilerCorrectness.entryPts_ok p p ExternIdents entrypoints),*),
-              Sim_inj.Forward_simulation_inject _ _ CSharpMin_CompcertCoreSem CMin_CompcertCoreSem
-                  ge tge entrypoints.
-Proof.
-  intros. eapply inj_simulation_star with ( match_state := match_cores)(order:=MC_order)(measure:=MC_measure).
-   apply MC_wellfounded.
-   intros. eapply init_cores; eauto.
+intros. apply   transl_program_correct. 
+(*Direct proof (literally the same as above theorem:
+apply inj_simulation_star with (match_states:=match_cores)(measure:=MC_measure).
+   intros. eapply (init_cores _ _ _ entrypoints); eauto.
    apply MC_safely_halted.
-   eapply MC_at_external; eauto.
-    Focus 4.
+   apply MC_at_external.
+   apply  MC_after_external.
+  apply MS_step.*)
+Qed.
+
+End TRANSLATION.
